Linglib.lean
@@ -2992,3 +2992,4 @@ import Linglib.Data.Examples.Anderson2006b
 import Linglib.Data.Examples.Ariel2001
 import Linglib.Data.Examples.AsherLascarides2003
 import Linglib.Data.Examples.AssmannEtAl2023
+import Linglib.Data.Examples.Asudeh2022
